## Goal
Given integers $a$ and $b$, with **not both zero**, we want to compute $\gcd(a,b)$.

The **Euclidean Algorithm** efficiently computes the gcd by repeated application of the **Division Algorithm**.

---

# The Euclidean Algorithm (Process)

Given $a$ and $b$, assume $a \ge b > 0$.  
Apply the Division Algorithm repeatedly:

$$
a = bq_1 + r_1, \qquad 0 \le r_1 < b,
$$

$$
b = r_1 q_2 + r_2, \qquad 0 \le r_2 < r_1,
$$

$$
r_1 = r_2 q_3 + r_3, \qquad 0 \le r_3 < r_2,
$$

Continue:

$$
r_2 = r_3 q_4 + r_4,
$$
$$
r_3 = r_4 q_5 + r_5,
$$
and so on.

Eventually, since the remainders strictly decrease and are nonnegative integers, the process must stop:

$$
r_{k-2} = r_{k-1} q_k + r_k, \qquad 0 \le r_k < r_{k-1},
$$
$$
r_{k-1} = r_k q_{k+1} + 0.
$$

The sequence of remainders ends when we reach **zero**.

The **last non-zero** remainder, $r_k$, is the gcd.

---

# Key Lemma (Crucial Justification)

**Lemma.**  
If $a = bq + r$, then  
$$
\gcd(a,b) = \gcd(b,r).
$$

## Proof

Let $d = \gcd(a,b)$.

Since $d \mid a$ and $d \mid b$,  
then $d$ divides any linear combination:
$$
a - bq = r.
$$

Thus:
$$
d \mid r.
$$

So $d$ divides both $b$ and $r$.  
Thus $d$ is a **common divisor** of $b$ and $r$.

Conversely, if $c$ is any common divisor of $b$ and $r$, then

- $c \mid b$,  
- $c \mid r$,  
⇒ $c \mid (bq + r) = a$.

So $c$ divides both $a$ and $b$, and so $c \le d$.

Therefore:
$$
\gcd(a,b) = \gcd(b,r).
$$

This lemma allows us to replace a pair $(a,b)$ by $(b,r)$ without changing the gcd.

---

# Main Result

Because at each stage
$$
\gcd(a,b) = \gcd(b,r_1) = \gcd(r_1, r_2) = \cdots = \gcd(r_{k-1}, r_k),
$$
and finally
$$
\gcd(r_{k-1}, r_k) = \gcd(r_k, 0) = r_k,
$$
the **last non-zero remainder** is the gcd.

---

# Full Example  
Compute $\gcd(12378, 3054)$.

Let $a = 12378$ and $b = 3054$.

Apply the Euclidean Algorithm:

$$
12378 = 4 \cdot 3054 + 162
$$

$$
3054 = 18 \cdot 162 + 138
$$

$$
162 = 1 \cdot 138 + 24
$$

$$
138 = 5 \cdot 24 + 18
$$

$$
24 = 1 \cdot 18 + 6
$$

$$
18 = 3 \cdot 6 + 0
$$

Thus:
$$
\gcd(12378, 3054) = 6.
$$

---

# Extended Euclidean Algorithm (Back-Substitution)

We now express $6$ as a linear combination of $12378$ and $3054$.

Starting from the second-to-last equation:

1.  
$$
6 = 24 - 1 \cdot 18
$$

2. Substitute $18$ from  
$$18 = 138 - 5 \cdot 24$$  
giving:
$$
6 = 24 - \big(138 - 5 \cdot 24\big)
= 6\cdot 24 - 138
$$

3. Substitute $24$ from  
$$24 = 162 - 1 \cdot 138$$  
giving:
$$
6 = 6(162 - 138) - 138
= 6 \cdot 162 - 7 \cdot 138
$$

4. Substitute $138$ from  
$$138 = 3054 - 18 \cdot 162$$  
giving:
$$
6 = 6 \cdot 162 - 7(3054 - 18 \cdot 162)
$$
$$
6 = 6\cdot 162 - 7\cdot 3054 + 126\cdot 162
$$
$$
6 = 132 \cdot 162 - 7 \cdot 3054
$$

5. Substitute $162$ from  
$$162 = 12378 - 4 \cdot 3054$$  
giving:
$$
6 = 132(12378 - 4 \cdot 3054) - 7 \cdot 3054
$$

Expand:
$$
6 = 132 \cdot 12378 - 528 \cdot 3054 - 7 \cdot 3054
$$

Combine like terms:
$$
6 = 132 \cdot 12378 + (-535) \cdot 3054
$$

Thus:
$$
6 = \gcd(12378,3054) = 12378(132) + 3054(-535).
$$

So the Bézout coefficients are:
- $x = 132$  
- $y = -535$

---
